src/Init/Data/String/Lemmas/Pattern/Pred.lean
@@ -181,43 +181,39 @@ theorem dropPrefix?_prop_eq_dropPrefix?_decide {p : Char → Prop} [DecidablePre
 theorem dropPrefix_prop_eq_dropPrefix_decide {p : Char → Prop} [DecidablePred p] {s : Slice} :
     s.dropPrefix p = s.dropPrefix (decide <| p ·) := (rfl)
 
+theorem skipPrefix?_prop_eq_skipPrefix?_decide {p : Char → Prop} [DecidablePred p] {s : Slice} :
+    s.skipPrefix? p = s.skipPrefix? (decide <| p ·) := (rfl)
+
 theorem Pattern.ForwardPattern.skipPrefix?_prop_eq_skipPrefix?_decide
     {p : Char → Prop} [DecidablePred p] {s : Slice} :
     skipPrefix? p s = skipPrefix? (decide <| p ·) s := (rfl)
 
-private theorem dropWhileGo_eq {p : Char → Prop} [DecidablePred p] {s : Slice} (curr : s.Pos) :
-    dropWhile.go s p curr = dropWhile.go s (decide <| p ·) curr := by
-  fun_induction dropWhile.go s p curr with
+theorem Pos.skipWhile_prop_eq_skipWhile_decide {p : Char → Prop} [DecidablePred p] {s : Slice}
+    (curr : s.Pos) :
+    Pos.skipWhile curr p = Pos.skipWhile curr (decide <| p ·) := by
+  fun_induction Pos.skipWhile curr p with
   | case1 pos nextCurr h₁ h₂ ih =>
-    conv => rhs; rw [dropWhile.go]
+    conv => rhs; rw [Pos.skipWhile]
     simp [← Pattern.ForwardPattern.skipPrefix?_prop_eq_skipPrefix?_decide, h₁, h₂, ih]
   | case2 pos nextCurr h ih =>
-    conv => rhs; rw [dropWhile.go]
+    conv => rhs; rw [Pos.skipWhile]
     simp [← Pattern.ForwardPattern.skipPrefix?_prop_eq_skipPrefix?_decide, h, ih]
   | case3 pos h =>
-    conv => rhs; rw [dropWhile.go]
+    conv => rhs; rw [Pos.skipWhile]
     simp [← Pattern.ForwardPattern.skipPrefix?_prop_eq_skipPrefix?_decide]
+
+theorem skipPrefixWhile_prop_eq_skipPrefixWhile_decide {p : Char → Prop} [DecidablePred p]
+    {s : Slice} :
+    s.skipPrefixWhile p = s.skipPrefixWhile (decide <| p ·) :=
+  Pos.skipWhile_prop_eq_skipWhile_decide s.startPos
 
 theorem dropWhile_prop_eq_dropWhile_decide {p : Char → Prop} [DecidablePred p] {s : Slice} :
     s.dropWhile p = s.dropWhile (decide <| p ·) := by
-  simpa only [dropWhile] using dropWhileGo_eq s.startPos
-
-private theorem takeWhileGo_eq {p : Char → Prop} [DecidablePred p] {s : Slice} (curr : s.Pos) :
-    takeWhile.go s p curr = takeWhile.go s (decide <| p ·) curr := by
-  fun_induction takeWhile.go s p curr with
-  | case1 pos nextCurr h₁ h₂ ih =>
-    conv => rhs; rw [takeWhile.go]
-    simp [← Pattern.ForwardPattern.skipPrefix?_prop_eq_skipPrefix?_decide, h₁, h₂, ih]
-  | case2 pos nextCurr h ih =>
-    conv => rhs; rw [takeWhile.go]
-    simp [← Pattern.ForwardPattern.skipPrefix?_prop_eq_skipPrefix?_decide, h, ih]
-  | case3 pos h =>
-    conv => rhs; rw [takeWhile.go]
-    simp [← Pattern.ForwardPattern.skipPrefix?_prop_eq_skipPrefix?_decide]
+  simp only [dropWhile]; exact congrArg _ skipPrefixWhile_prop_eq_skipPrefixWhile_decide
 
 theorem takeWhile_prop_eq_takeWhile_decide {p : Char → Prop} [DecidablePred p] {s : Slice} :
     s.takeWhile p = s.takeWhile (decide <| p ·) := by
-  simp only [takeWhile]; exact takeWhileGo_eq s.startPos
+  simp only [takeWhile]; exact congrArg _ skipPrefixWhile_prop_eq_skipPrefixWhile_decide
 
 theorem all_prop_eq_all_decide {p : Char → Prop} [DecidablePred p] {s : Slice} :
     s.all p = s.all (decide <| p ·) := by
@@ -239,52 +235,46 @@ theorem contains_prop_eq_contains_decide {p : Char → Prop} [DecidablePred p] {
 theorem endsWith_prop_eq_endsWith_decide {p : Char → Prop} [DecidablePred p] {s : Slice} :
     s.endsWith p = s.endsWith (decide <| p ·) := (rfl)
 
+theorem skipSuffix?_prop_eq_skipSuffix?_decide {p : Char → Prop} [DecidablePred p] {s : Slice} :
+    s.skipSuffix? p = s.skipSuffix? (decide <| p ·) := (rfl)
+
 theorem dropSuffix?_prop_eq_dropSuffix?_decide {p : Char → Prop} [DecidablePred p] {s : Slice} :
     s.dropSuffix? p = s.dropSuffix? (decide <| p ·) := (rfl)
 
 theorem dropSuffix_prop_eq_dropSuffix_decide {p : Char → Prop} [DecidablePred p] {s : Slice} :
     s.dropSuffix p = s.dropSuffix (decide <| p ·) := (rfl)
 
-theorem Pattern.BackwardPattern.dropSuffix?_prop_eq_dropSuffix?_decide
+theorem Pattern.BackwardPattern.skipSuffix?_prop_eq_skipSuffix?_decide
     {p : Char → Prop} [DecidablePred p] {s : Slice} :
-    dropSuffix? p s = dropSuffix? (decide <| p ·) s := (rfl)
+    skipSuffix? p s = skipSuffix? (decide <| p ·) s := (rfl)
 
-private theorem dropEndWhileGo_eq {p : Char → Prop} [DecidablePred p] {s : Slice}
-    (curr : s.Pos) :
-    dropEndWhile.go s p curr = dropEndWhile.go s (decide <| p ·) curr := by
-  fun_induction dropEndWhile.go s p curr with
+theorem Pos.revSkipWhile_prop_eq_revSkipWhile_decide {p : Char → Prop} [DecidablePred p]
+    {s : Slice} (curr : s.Pos) :
+    Pos.revSkipWhile curr p = Pos.revSkipWhile curr (decide <| p ·) := by
+  fun_induction Pos.revSkipWhile curr p with
   | case1 pos nextCurr h₁ h₂ ih =>
-    conv => rhs; rw [dropEndWhile.go]
-    simp [← Pattern.BackwardPattern.dropSuffix?_prop_eq_dropSuffix?_decide, h₁, h₂, ih]
+    conv => rhs; rw [Pos.revSkipWhile]
+    simp [← Pattern.BackwardPattern.skipSuffix?_prop_eq_skipSuffix?_decide, h₁, h₂, ih]
   | case2 pos nextCurr h ih =>
-    conv => rhs; rw [dropEndWhile.go]
-    simp [← Pattern.BackwardPattern.dropSuffix?_prop_eq_dropSuffix?_decide, h, ih]
+    conv => rhs; rw [Pos.revSkipWhile]
+    simp [← Pattern.BackwardPattern.skipSuffix?_prop_eq_skipSuffix?_decide, h, ih]
   | case3 pos h =>
-    conv => rhs; rw [dropEndWhile.go]
-    simp [← Pattern.BackwardPattern.dropSuffix?_prop_eq_dropSuffix?_decide]
+    conv => rhs; rw [Pos.revSkipWhile]
+    simp [← Pattern.BackwardPattern.skipSuffix?_prop_eq_skipSuffix?_decide]
+
+theorem skipSuffixWhile_prop_eq_skipSuffixWhile_decide {p : Char → Prop} [DecidablePred p]
+    {s : Slice} :
+    s.skipSuffixWhile p = s.skipSuffixWhile (decide <| p ·) :=
+  Pos.revSkipWhile_prop_eq_revSkipWhile_decide s.endPos
 
 theorem dropEndWhile_prop_eq_dropEndWhile_decide {p : Char → Prop} [DecidablePred p]
     {s : Slice} :
     s.dropEndWhile p = s.dropEndWhile (decide <| p ·) := by
-  simpa only [dropEndWhile] using dropEndWhileGo_eq s.endPos
-
-private theorem takeEndWhileGo_eq {p : Char → Prop} [DecidablePred p] {s : Slice}
-    (curr : s.Pos) :
-    takeEndWhile.go s p curr = takeEndWhile.go s (decide <| p ·) curr := by
-  fun_induction takeEndWhile.go s p curr with
-  | case1 pos nextCurr h₁ h₂ ih =>
-    conv => rhs; rw [takeEndWhile.go]
-    simp [← Pattern.BackwardPattern.dropSuffix?_prop_eq_dropSuffix?_decide, h₁, h₂, ih]
-  | case2 pos nextCurr h ih =>
-    conv => rhs; rw [takeEndWhile.go]
-    simp [← Pattern.BackwardPattern.dropSuffix?_prop_eq_dropSuffix?_decide, h, ih]
-  | case3 pos h =>
-    conv => rhs; rw [takeEndWhile.go]
-    simp [← Pattern.BackwardPattern.dropSuffix?_prop_eq_dropSuffix?_decide]
+  simp only [dropEndWhile]; exact congrArg _ skipSuffixWhile_prop_eq_skipSuffixWhile_decide
 
 theorem takeEndWhile_prop_eq_takeEndWhile_decide {p : Char → Prop} [DecidablePred p]
     {s : Slice} :
     s.takeEndWhile p = s.takeEndWhile (decide <| p ·) := by
-  simpa only [takeEndWhile] using takeEndWhileGo_eq s.endPos
+  simp only [takeEndWhile]; exact congrArg _ skipSuffixWhile_prop_eq_skipSuffixWhile_decide
 
 end String.Slice
